Get rid of lookup

Launchbury/Env.thy
@@ -10,42 +10,27 @@ type_synonym  ('a, 'b) fmap = "'a \<Rightarrow> 'b" (infixr "f\<rightharpoonup>"
 
 definition fdom :: "'key f\<rightharpoonup> 'value::pcpo \<Rightarrow> 'key set" where "fdom m = {x. m x \<noteq> \<bottom>}"
 
-definition lookup :: "'key f\<rightharpoonup> 'value \<Rightarrow> 'key \<Rightarrow> 'value" (infix "f!" 55) where "lookup m x = m x"
-
-lemma lookup_fempty[simp]: "lookup \<bottom> x = \<bottom>" by (simp add: lookup_def)
-
 lemma fempty_fdom[simp]: "fdom \<bottom> = {}" by (simp add: fdom_def)
 
 lemma fempty_fdom2[simp]: "fdom (\<lambda>_ . \<bottom>) = {}" by (simp add: fdom_def)
 
-lemma fdomIff: "(a \<in> fdom m) = (lookup m a \<noteq> \<bottom>)" by (simp add: fdom_def lookup_def)
+lemma fdomIff: "(a \<in> fdom m) = (m a \<noteq> \<bottom>)" by (simp add: fdom_def)
 
-lemma lookup_not_fdom: "x \<notin> fdom m \<Longrightarrow> lookup m x = \<bottom>"  by (auto iff:fdomIff)
+lemma lookup_not_fdom: "x \<notin> fdom m \<Longrightarrow> m x = \<bottom>"  by (auto iff:fdomIff)
 
-lemma lookup_fdom[simp]: "m f! x \<noteq> \<bottom> \<Longrightarrow> x \<in> fdom m"  by (auto iff:fdomIff)
-
-lemma fmap_eqI:
-  assumes "\<And> x. a f! x = b f! x"
-  shows "a = b"
-using assms
-by (auto simp add: lookup_def)
+lemma lookup_fdom[simp]: "m x \<noteq> \<bottom> \<Longrightarrow> x \<in> fdom m"  by (auto iff:fdomIff)
 
 subsubsection {* Updates *}
 
 lemma fdom_fun_upd_subset: "fdom (h (x := v)) \<subseteq> insert x (fdom h)"
   by (auto simp add: fdom_def)
 
-lemma lookup_fun_upd[simp]: "lookup (h (x := v)) x = v"
-  by (auto simp add: fdom_def  lookup_def)
+declare fun_upd_same[simp] fun_upd_other[simp]
 
-lemma lookup_fun_upd_other[simp]: "x' \<noteq> x \<Longrightarrow> lookup (h (x := v)) x' = lookup h x'"
-  by (auto simp add: fdom_def  lookup_def)
-
-lemma lookup_fun_upd_eq: "lookup (h (x := v)) x' = (if x = x' then v else lookup h x')"
-  by (auto simp add: fdom_def  lookup_def)
-
-lemma fun_upd_noop[simp]: "x \<in> fdom f \<Longrightarrow> y = f f! x \<Longrightarrow> f (x := y) = f"
-  by (auto simp add: fdom_def  lookup_def)
+(*
+lemma fun_upd_noop[simp]: "x \<in> fdom f \<Longrightarrow> y = f  x \<Longrightarrow> f (x := y) = f"
+  by (auto simp add: fdom_def )
+*)
 
 lemma fun_upd_eqD1: "m(a := x) = n(a := y) \<Longrightarrow> x = y"
   by (metis fun_upd_same)
@@ -60,43 +45,42 @@ abbreviation fmap_restr_rev  (infixl "f|`"  110) where "fmap_restr_rev m S \<equ
 lemma fmap_restr_empty[simp]: "fdom m \<inter> S = {} \<Longrightarrow> m f|` S = \<bottom>"
   by (fastforce simp add: fdom_def fmap_restr_def)
 
-lemma lookup_fmap_restr[simp]: "x \<in> S \<Longrightarrow> lookup (fmap_restr S m) x = lookup m x"
-  by (fastforce simp add: fmap_restr_def lookup_def)
+lemma lookup_fmap_restr[simp]: "x \<in> S \<Longrightarrow> (fmap_restr S m) x = m x"
+  by (fastforce simp add: fmap_restr_def)
 
-lemma lookup_fmap_restr_not_there[simp]: "x \<notin> S \<Longrightarrow> lookup (fmap_restr S m) x = \<bottom>"
-  by (fastforce simp add: fmap_restr_def lookup_def)
+lemma lookup_fmap_restr_not_there[simp]: "x \<notin> S \<Longrightarrow> (fmap_restr S m) x = \<bottom>"
+  by (fastforce simp add: fmap_restr_def)
 
-lemma lookup_fmap_restr_eq: "m f|` S f! x = (if x \<in> S then m f! x else \<bottom>)"
-  by (simp)
-
+lemma lookup_fmap_restr_eq: "(m f|` S) x = (if x \<in> S then m x else \<bottom>)"
+  by simp
 
 lemma fmap_restr_cong: "fdom m \<inter> S1 = fdom m \<inter> S2 \<Longrightarrow> m f|` S1 = m f|` S2"
-  apply (rule fmap_eqI)
+  apply (rule ext)
   apply (simp add: lookup_fmap_restr_eq)
   by (metis Int_iff lookup_not_fdom)
 
 lemma fmap_restr_fmap_restr[simp]:
  "x f|` d2 f|` d1 = x f|` (d1 \<inter> d2)"
-  by (fastforce simp add: fmap_restr_def lookup_def)
+  by (fastforce simp add: fmap_restr_def)
 
 lemma fmap_restr_fmap_restr_subset:
  "d1 \<subseteq> d2 \<Longrightarrow> x f|` d2 f|` d1 = x f|` d1"
  by (metis Int_absorb2 fmap_restr_fmap_restr)
 
 lemma fmap_restr_useless: "fdom m \<subseteq> S \<Longrightarrow> m f|` S = m"
-  by (rule fmap_eqI) (auto simp add: lookup_fmap_restr_eq dest!: set_mp)
+  by (rule ext) (auto simp add: lookup_fmap_restr_eq dest!: set_mp)
 
 lemma fmap_restr_UNIV[simp]: "m f|` UNIV = m"
   by (rule fmap_restr_useless) simp
 
 lemma fmap_restr_fun_upd[simp]: "x \<in> S \<Longrightarrow> m1(x := v) f|` S = (m1 f|` S)(x := v)"
-  apply (rule fmap_eqI)
+  apply (rule ext)
   apply (case_tac "xa = x")
   apply (auto simp add: lookup_fmap_restr_eq)
   done
 
 lemma fmap_restr_fun_upd_other[simp]: "x \<notin> S \<Longrightarrow> m1(x := v) f|` S = m1 f|` S"
-  apply (rule fmap_eqI)
+  apply (rule ext)
   apply (case_tac "xa = x")
   apply (auto simp add: lookup_fmap_restr_eq)
   done
@@ -107,46 +91,46 @@ definition fmap_delete :: "'a \<Rightarrow> 'a f\<rightharpoonup> 'b \<Rightarro
   where "fmap_delete x m = m(x := \<bottom>)"
 
 lemma lookup_fmap_delete[simp]:
-  "x' \<noteq> x \<Longrightarrow> fmap_delete x m f! x' = m f! x'"
-  by (simp add: fmap_delete_def lookup_def)
+  "x' \<noteq> x \<Longrightarrow> fmap_delete x m x' = m x'"
+  by (simp add: fmap_delete_def)
 
 lemma lookup_fmap_delete_None[simp]:
-  "fmap_delete x m f! x = \<bottom>"
-  by (simp add: fmap_delete_def lookup_def)
+  "fmap_delete x m x = \<bottom>"
+  by (simp add: fmap_delete_def)
 
 lemma fdom_fmap_delete[simp]:
   "fdom (fmap_delete x m) = fdom m - {x}"
-  by (auto simp add: fmap_delete_def lookup_def fdom_def)
+  by (auto simp add: fmap_delete_def fdom_def)
 
 lemma fdom_fmap_delete_subset:
   "fdom (fmap_delete x m) \<subseteq> fdom m" by auto
 
 lemma fmap_delete_fun_upd[simp]:
   "fmap_delete x (m(x := v)) = fmap_delete x m"
-  by (auto simp add: fmap_delete_def )
+  by (auto simp add: fmap_delete_def)
 
 lemma fmap_delete_fun_upd2[simp]:
   "(fmap_delete x m)(x := v) = m(x := v)"
-  by (auto simp add: fmap_delete_def )
+  by (auto simp add: fmap_delete_def)
 
 lemma fmap_delete_fun_upd3[simp]:
   "x \<noteq> y \<Longrightarrow> fmap_delete x (m(y := v)) = (fmap_delete x m)(y := v)"
-  by (auto simp add: fmap_delete_def )
+  by (auto simp add: fmap_delete_def)
 
 lemma fmap_delete_noop[simp]:
   "x \<notin> fdom m \<Longrightarrow> fmap_delete x m = m"
   by (auto simp add: fmap_delete_def fdom_def)
 
-lemma fun_upd_fmap_delete[simp]: "x \<in> fdom \<Gamma> \<Longrightarrow> (fmap_delete x \<Gamma>)(x := \<Gamma> f! x) = \<Gamma>"
+lemma fun_upd_fmap_delete[simp]: "x \<in> fdom \<Gamma> \<Longrightarrow> (fmap_delete x \<Gamma>)(x := \<Gamma> x) = \<Gamma>"
   by (auto)
 
 lemma fmap_restr_fmap_delete_other[simp]: "x \<notin> S \<Longrightarrow> fmap_delete x m f|` S = m f|` S"
-  apply (rule fmap_eqI)
+  apply (rule ext)
   apply (auto simp add: lookup_fmap_restr_eq)
   by (metis lookup_fmap_delete)
 
 lemma fmap_delete_restr: "fmap_delete x m = m f|` (-{x})"
-  by (auto intro: fmap_eqI simp add: lookup_fmap_restr_eq)
+  by (auto simp add: lookup_fmap_restr_eq)
 
 subsubsection {* Addition (merging) of finite maps *}
 
@@ -156,36 +140,36 @@ definition fmap_add :: "'a set \<Rightarrow> 'a f\<rightharpoonup> 'b \<Rightarr
 abbreviation fmap_add_syn ("_ f++\<^bsub>_\<^esub> _" [100, 0, 100] 100) where "f1 f++\<^bsub>S\<^esub> f2 \<equiv> fmap_add S f1 f2"
 
 lemma fmap_add_fempty[simp]: "\<bottom> f++\<^bsub>S\<^esub> m = m f|` S" 
-  by (auto simp add: fmap_add_def lookup_def fmap_restr_def)
+  by (auto simp add: fmap_add_def fmap_restr_def)
 
 lemma fmap_add_fempty2[simp]: "m f++\<^bsub>S\<^esub> \<bottom> = m f|` (-S)" 
-  by (auto simp add: fmap_add_def lookup_def fmap_restr_def)
+  by (auto simp add: fmap_add_def fmap_restr_def)
 
 lemma fdom_fmap_add[simp]: "fdom (m1 f++\<^bsub>S\<^esub> m2) = (fdom m1 - S) \<union> (fdom m2 \<inter> S)"
-  by (auto simp add: fmap_add_def lookup_def fdom_def)
+  by (auto simp add: fmap_add_def fdom_def)
 
-lemma lookup_fmap_add1[simp]: "x \<in> S \<Longrightarrow> m1 f++\<^bsub>S\<^esub> m2 f! x = m2 f! x"
-  by (auto simp add: fmap_add_def lookup_def fdom_def)
+lemma lookup_fmap_add1[simp]: "x \<in> S \<Longrightarrow> (m1 f++\<^bsub>S\<^esub> m2) x = m2 x"
+  by (auto simp add: fmap_add_def fdom_def)
 
-lemma lookup_fmap_add2[simp]:  "x \<notin> S \<Longrightarrow>  m1 f++\<^bsub>S\<^esub> m2 f! x = m1 f! x"
-  by (auto simp add: fmap_add_def lookup_def fdom_def)
+lemma lookup_fmap_add2[simp]:  "x \<notin> S \<Longrightarrow> (m1 f++\<^bsub>S\<^esub> m2) x = m1 x"
+  by (auto simp add: fmap_add_def fdom_def)
 
-lemma lookup_fmap_add_eq: " m1 f++\<^bsub>S\<^esub> m2 f! x = (if x \<in> S then m2 f! x else m1 f! x)"
+lemma lookup_fmap_add_eq: "(m1 f++\<^bsub>S\<^esub> m2) x = (if x \<in> S then m2 x else m1 x)"
   by (cases "x \<notin> S") simp_all
 
 lemma fmap_add_upd_swap: 
   "x \<notin> S \<Longrightarrow> \<rho>(x := z) f++\<^bsub>S\<^esub> \<rho>' = (\<rho> f++\<^bsub>S\<^esub> \<rho>')(x := z)"
-  by (auto simp add: fmap_add_def  lookup_def fdom_def)
+  by (auto simp add: fmap_add_def  fdom_def)
 
 lemma fmap_add_upd: 
   "x \<in> S \<Longrightarrow> \<rho> f++\<^bsub>S\<^esub> (\<rho>'(x := z)) = (\<rho> f++\<^bsub>S - {x}\<^esub> \<rho>')(x := z)"
-  by (auto simp add: fmap_add_def  lookup_def fdom_def)
+  by (auto simp add: fmap_add_def  fdom_def)
 
 lemma fmap_restr_add: "fmap_restr S (m1 f++\<^bsub>S2\<^esub> m2) = fmap_restr S m1 f++\<^bsub>S2\<^esub> fmap_restr S m2"
-  by (auto simp add: fmap_add_def  lookup_def fdom_def fmap_restr_def)
+  by (auto simp add: fmap_add_def  fdom_def fmap_restr_def)
 
 lemma fmap_delete_add: "fmap_delete x (m1 f++\<^bsub>S\<^esub> m2) = fmap_delete x m1 f++\<^bsub>S - {x}\<^esub> fmap_delete x m2"
-  by (auto simp add: fmap_add_def  lookup_def fdom_def fmap_restr_def fmap_delete_def)
+  by (auto simp add: fmap_add_def  fdom_def fmap_restr_def fmap_delete_def)
 
 subsubsection {* Map *}
 
@@ -193,20 +177,21 @@ definition fmap_map :: "('b \<Rightarrow> 'c) \<Rightarrow> 'a f\<rightharpoonup
 
 lemma fmap_map_id[simp]: "fmap_map (\<lambda> x. x) m = m" by (simp add: fmap_map_def)
 
-lemma lookup_fmap_map[simp]: "lookup (fmap_map f m) x = f (lookup m x)"  by (simp add: fmap_map_def lookup_def)
+lemma lookup_fmap_map[simp]: "(fmap_map f m) x = f (m x)"  by (simp add: fmap_map_def)
 
 lemma fmap_map_fmap_restr[simp]: "f \<bottom> = \<bottom> \<Longrightarrow> fmap_map f (fmap_restr S m) = fmap_restr S (fmap_map f m)"
-  by (rule fmap_eqI) (auto simp add: lookup_fmap_restr_eq)
+  by (rule ext) (auto simp add: lookup_fmap_restr_eq)
 
 lemma fmap_map_fun_upd[simp]: "fmap_map f (m(x := v)) = (fmap_map f m)(x := f v)"
-  by (auto simp add: fmap_map_def lookup_def )
+  by (auto simp add: fmap_map_def  )
 
 
 subsection {* Lifting relations pointwise *}
 
-inductive fmap_lift_rel for P where
-  fmap_lift_relI[intro]: "(\<And> x. P (m f! x) (m' f! x)) \<Longrightarrow> fmap_lift_rel P m m'"
-
+definition pointwise where "pointwise P m m' = (\<forall> x. P (m x) (m' x))"
+lemma pointwiseI[intro]: "(\<And> x. P (m x) ( m' x)) \<Longrightarrow> pointwise P m m'" unfolding pointwise_def by blast
+(*
 inductive_cases fmap_lift_relE[elim]:  "fmap_lift_rel P m m'" 
+*)
 
 end
