Launchbury/HeapToEnv.thy
@@ -19,7 +19,7 @@ lemma cont2cont_heapToEnv[simp, cont2cont]:
 
 lemma heapToEnv_eqvt[eqvt]:
   "\<pi> \<bullet> heapToEnv h eval = heapToEnv (\<pi> \<bullet> h) (\<pi> \<bullet> eval)"
-  by (induct h eval rule:heapToEnv.induct) (auto simp add:fun_upd_eqvt  lookup_def simp del: fun_upd_apply)
+  by (induct h eval rule:heapToEnv.induct) (auto simp add:fun_upd_eqvt  simp del: fun_upd_apply)
 
 lemma fdom_heapToEnv_subset:"fdom (heapToEnv h eval) \<subseteq> heapVars h"
   by (induct h eval rule:heapToEnv.induct) (auto dest:set_mp[OF fdom_fun_upd_subset] simp del: fun_upd_apply)
@@ -31,7 +31,7 @@ lemma heapToEnv_cong[fundef_cong]:
 
 lemma lookupHeapToEnv:
   assumes "v \<in> heapVars h"
-  shows "(heapToEnv h f) f! v = f (the (map_of h v))"
+  shows "(heapToEnv h f) v = f (the (map_of h v))"
   using assms
   apply (induct h)
   apply simp
@@ -41,7 +41,7 @@ lemma lookupHeapToEnv:
 
 lemma lookupHeapToEnv_other[simp]:
   assumes "v \<notin> heapVars h"
-  shows "(heapToEnv h f) f! v = \<bottom>"
+  shows "(heapToEnv h f) v = \<bottom>"
   using assms
   apply (induct h)
   apply simp
@@ -52,7 +52,7 @@ lemma lookupHeapToEnv_other[simp]:
 
 lemma fmap_restr_heapToEnv_noop:
   "heapVars h \<subseteq> S \<Longrightarrow> fmap_restr S (heapToEnv h eval) = heapToEnv h eval"
-  apply (rule fmap_eqI)
+  apply (rule ext)
   apply (case_tac "x \<in> S")
   apply (auto simp add: lookupHeapToEnv intro: lookupHeapToEnv_other)
   done
@@ -60,28 +60,15 @@ lemma fmap_restr_heapToEnv_noop:
 lemma heapToEnv_cong':
   "\<lbrakk> (\<And> x. x \<in> heapVars heap \<Longrightarrow> eval1 (the (map_of heap x)) = eval2 (the (map_of heap x))) \<rbrakk>
     \<Longrightarrow>  heapToEnv heap eval1 = heapToEnv heap eval2"
- apply (rule fmap_eqI)
+ apply (rule ext)
  apply (case_tac "x \<in> heapVars heap")
  apply (auto simp add: lookupHeapToEnv)
  done
 
 lemma lookupHeapToEnvNotAppend[simp]:
   assumes "x \<notin> heapVars \<Gamma>"
-  shows "heapToEnv (\<Gamma>@h) f f! x = heapToEnv h f f! x"
+  shows "(heapToEnv (\<Gamma>@h) f) x = heapToEnv h f x"
   using assms by (induct \<Gamma>, auto)
-
-(*
-lemma heapToEnv_remove_Cons_fmap_expand:
-  "finite S \<Longrightarrow> x \<notin> S \<Longrightarrow> heapToEnv ((x, e) # \<Gamma>) eval\<^bsub>[S]\<^esub> = heapToEnv \<Gamma> eval\<^bsub>[S]\<^esub>"
-  apply (rule fmap_eqI)
-  apply simp
-  apply (subgoal_tac "xa \<noteq> x")
-  apply (case_tac "xa \<in> heapVars \<Gamma>")
-  apply simp
-  apply simp
-  apply auto
-  done
-*)
 
 lemma heapToEnv_delete[simp]: "heapToEnv (delete x \<Gamma>) eval = fmap_delete x (heapToEnv \<Gamma> eval)"
   by (induct \<Gamma>) auto
@@ -90,7 +77,7 @@ lemma heapToEnv_mono:
   "x \<notin> heapVars \<Gamma> \<Longrightarrow>
   heapToEnv \<Gamma> eval \<sqsubseteq> heapToEnv ((x, e) # \<Gamma>) eval"
    apply simp
-   apply (rule fmap_belowI)
+   apply (rule fun_belowI)
    apply (case_tac "xa \<in> heapVars \<Gamma>")
    apply (case_tac "xa = x")
    apply auto
@@ -101,12 +88,12 @@ subsubsection {* Reordering lemmas *}
 lemma heapToEnv_reorder:
   assumes "map_of \<Gamma> = map_of \<Delta>"
   shows "heapToEnv \<Gamma> h = heapToEnv \<Delta> h"
-proof (rule fmap_eqI)
+proof (rule ext)
   from assms
   have *: "heapVars \<Gamma> = heapVars \<Delta>" by (metis dom_map_of_conv_heapVars)
 
   fix x
-  show "heapToEnv \<Gamma> h f! x = heapToEnv \<Delta> h f! x" 
+  show "heapToEnv \<Gamma> h x = heapToEnv \<Delta> h x" 
     using assms(1) *
     apply (cases "x \<in> heapVars \<Gamma>")
     apply (auto simp add: lookupHeapToEnv)
